Eliminate FloatStamp
To remove the dependency on a sorry required for the code generation
of stamps, we have elected to temporarily remove the FloatStamp.

Graph/Stamp.thy
@@ -17,7 +17,7 @@ text_raw \<open>\Snip{Stamp}%\<close>
 datatype Stamp = 
   VoidStamp
   | IntegerStamp (stp_bits: nat) (stpi_lower: int) (stpi_upper: int)
-  | FloatStamp (stp_bits: nat) (stpf_lower: float) (stpf_upper: float)
+  (* | FloatStamp (stp_bits: nat) (stpf_lower: float) (stpf_upper: float) *)
   | KlassPointerStamp (stp_nonNull: bool) (stp_alwaysNull: bool)
   | MethodCountersPointerStamp (stp_nonNull: bool) (stp_alwaysNull: bool)
   | MethodPointersStamp (stp_nonNull: bool) (stp_alwaysNull: bool)
@@ -29,7 +29,7 @@ text_raw \<open>\EndSnip\<close>
 fun unrestricted_stamp :: "Stamp \<Rightarrow> Stamp" where
   "unrestricted_stamp VoidStamp = VoidStamp" |
   "unrestricted_stamp (IntegerStamp bits lower upper) = (IntegerStamp bits (fst (bit_bounds bits)) (snd (bit_bounds bits)))" | 
-  "unrestricted_stamp (FloatStamp bits lower upper) = (FloatStamp bits neg_infinity pos_infinity)" | 
+  (* "unrestricted_stamp (FloatStamp bits lower upper) = (FloatStamp bits neg_infinity pos_infinity)" |  *)
   "unrestricted_stamp (KlassPointerStamp nonNull alwaysNull) = (KlassPointerStamp False False)" |
   "unrestricted_stamp (MethodCountersPointerStamp nonNull alwaysNull) = (MethodCountersPointerStamp False False)" |
   "unrestricted_stamp (MethodPointersStamp nonNull alwaysNull) = (MethodPointersStamp False False)" |
@@ -42,7 +42,7 @@ fun is_stamp_unrestricted :: "Stamp \<Rightarrow> bool" where
 fun empty_stamp :: "Stamp \<Rightarrow> Stamp" where
   "empty_stamp VoidStamp = VoidStamp" |
   "empty_stamp (IntegerStamp bits lower upper) = (IntegerStamp bits (snd (bit_bounds bits)) (fst (bit_bounds bits)))" |
-  "empty_stamp (FloatStamp bits lower upper) = (FloatStamp bits pos_infinity neg_infinity)" |
+  (* "empty_stamp (FloatStamp bits lower upper) = (FloatStamp bits pos_infinity neg_infinity)" | *)
   "empty_stamp (KlassPointerStamp nonNull alwaysNull) = (KlassPointerStamp nonNull alwaysNull)" |
   "empty_stamp (MethodCountersPointerStamp nonNull alwaysNull) = (MethodCountersPointerStamp nonNull alwaysNull)" |
   "empty_stamp (MethodPointersStamp nonNull alwaysNull) = (MethodPointersStamp nonNull alwaysNull)" |
@@ -51,7 +51,7 @@ fun empty_stamp :: "Stamp \<Rightarrow> Stamp" where
 
 fun is_stamp_empty :: "Stamp \<Rightarrow> bool" where
   "is_stamp_empty (IntegerStamp b lower upper) = (upper < lower)" |
-  "is_stamp_empty (FloatStamp b lower upper) = (upper < lower)" |
+  (* "is_stamp_empty (FloatStamp b lower upper) = (upper < lower)" | *)
   "is_stamp_empty x = False"
 
 fun meet :: "Stamp \<Rightarrow> Stamp \<Rightarrow> Stamp" where
@@ -60,10 +60,10 @@ fun meet :: "Stamp \<Rightarrow> Stamp \<Rightarrow> Stamp" where
     if b1 \<noteq> b2 then IllegalStamp else 
     (IntegerStamp b1 (min l1 l2) (max u1 u2))
   )" |
-  "meet (FloatStamp b1 l1 u1) (FloatStamp b2 l2 u2) = (
+  (* "meet (FloatStamp b1 l1 u1) (FloatStamp b2 l2 u2) = (
     if b1 \<noteq> b2 then IllegalStamp else 
     (FloatStamp b1 (min l1 l2) (max u1 u2))
-  )" |
+  )" | *)
   "meet (KlassPointerStamp nn1 an1) (KlassPointerStamp nn2 an2) = (
     KlassPointerStamp (nn1 \<and> nn2) (an1 \<and> an2)
   )" |
@@ -81,10 +81,10 @@ fun join :: "Stamp \<Rightarrow> Stamp \<Rightarrow> Stamp" where
     if b1 \<noteq> b2 then IllegalStamp else 
     (IntegerStamp b1 (max l1 l2) (min u1 u2))
   )" |
-  "join (FloatStamp b1 l1 u1) (FloatStamp b2 l2 u2) = (
+  (* "join (FloatStamp b1 l1 u1) (FloatStamp b2 l2 u2) = (
     if b1 \<noteq> b2 then IllegalStamp else 
     (FloatStamp b1 (max l1 l2) (min u1 u2))
-  )" |
+  )" | *)
   "join (KlassPointerStamp nn1 an1) (KlassPointerStamp nn2 an2) = (
     if ((nn1 \<or> nn2) \<and> (an1 \<or> an2)) 
     then (empty_stamp (KlassPointerStamp nn1 an1))
@@ -120,7 +120,7 @@ fun constantAsStamp :: "Value \<Rightarrow> Stamp" where
 
 fun valid_value :: "Stamp \<Rightarrow> Value \<Rightarrow> bool" where
   "valid_value (IntegerStamp b1 l h) (IntVal b2 v) = ((b1 = b2) \<and> (v \<ge> l) \<and> (v \<le> h))" |
-  "valid_value (FloatStamp b1 l h) (FloatVal b2 v) = ((b1 = b2) \<and> (v \<ge> l) \<and> (v \<le> h))" |
+  (* "valid_value (FloatStamp b1 l h) (FloatVal b2 v) = ((b1 = b2) \<and> (v \<ge> l) \<and> (v \<le> h))" | *)
   "valid_value (VoidStamp) (UndefVal) = True" |
   "valid_value stamp val = False"
 
@@ -134,18 +134,20 @@ lemma int_valid_range:
   using assms valid_value.simps apply auto
   using valid_value.elims(2) by blast
 
+(*
 lemma float_valid_range:
   assumes "stamp = FloatStamp bits lower upper"
   shows "{x . valid_value stamp x} = {(FloatVal bits val) | val . val \<in> {lower..upper}}"
   using assms valid_value.simps apply auto
   using valid_value.simps
   by (metis less_eq_float.rep_eq valid_value.elims(2))
+*)
 
 lemma disjoint_empty:
   assumes "joined = (join x_stamp y_stamp)"
   assumes "is_stamp_empty joined"
   shows "{x . valid_value x_stamp x} \<inter> {y . valid_value y_stamp y} = {}"
-  using assms int_valid_range float_valid_range
+  using assms int_valid_range (*float_valid_range*)
   by (induction "x_stamp"; induction "y_stamp"; auto)
 
 lemma join_unequal:
@@ -190,12 +192,12 @@ lemma boundsAlwaysOverlap:
 lemma intstamp_bits_eq_meet:
   assumes "(meet (IntegerStamp b1 l1 u1) (IntegerStamp b2 l2 u2)) = (IntegerStamp b3 l3 u3)"
   shows "b1 = b3 \<and> b2 = b3"
-  by (metis Stamp.distinct(29) assms meet.simps(2))
+  by (metis Stamp.distinct(25) assms meet.simps(2))
 
 lemma intstamp_bits_eq_join:
   assumes "(join (IntegerStamp b1 l1 u1) (IntegerStamp b2 l2 u2)) = (IntegerStamp b3 l3 u3)"
   shows "b1 = b3 \<and> b2 = b3"
-  by (metis Stamp.distinct(29) assms join.simps(2))
+  by (metis Stamp.distinct(25) assms join.simps(2))
 
 lemma intstamp_bites_eq_unrestricted:
   assumes "(unrestricted_stamp (IntegerStamp b1 l1 u1)) = (IntegerStamp b2 l2 u2)"
@@ -207,6 +209,7 @@ lemma intstamp_bits_eq_empty:
   shows "b1 = b2"
   using assms by auto
 
+(*
 lemma floatstamp_bits_eq_meet:
   assumes "(meet (FloatStamp b1 l1 u1) (FloatStamp b2 l2 u2)) = (FloatStamp b3 l3 u3)"
   shows "b1 = b3 \<and> b2 = b3"
@@ -226,6 +229,7 @@ lemma floatstamp_bits_eq_empty:
   assumes "(empty_stamp (FloatStamp b1 l1 u1)) = (FloatStamp b2 l2 u2)"
   shows "b1 = b2"
   using assms by auto
+*)
 
 (* Manual sanity checks *)
 notepad
@@ -248,6 +252,7 @@ begin
     by auto
 end
 
+(*
 notepad
 begin
   have "unrestricted_stamp (FloatStamp 8 0 10) = (FloatStamp 8 neg_infinity pos_infinity)"
@@ -267,5 +272,6 @@ begin
   have "meet (FloatStamp 32 0 20) (FloatStamp 32 (-100) 10) = (FloatStamp 32 (- 100) 20)"
     by auto
 end
+*)
 
 end
